adding terms + lemma 4.2 hypothesis + some hash dev

src/IsoCan.v
@@ -7,36 +7,119 @@ From RDF Require Import Rdf Triple Term.
 (* From Coq Require Import List. *)
 
 
-
-
 Section IsoCan.
   (* Axiom todo : forall A,A. *)
   Variable I B L: eqType.
   Let rdf_graph:= (rdf_graph I B L).
   Let triple:= (triple I B L).
   Let term:= (term I B L).
-  Let relabeling:= (Rdf.relabeling).
 
   Definition isocanonical_function (M : B -> B) (g : rdf_graph) :=
     iso g (Rdf.relabeling M g) /\
       forall (h : rdf_graph), iso g h <-> (relabeling M g) = (relabeling M h).
 
   Section IsoCanAlgorithm.
-    Variable hash : eqType.
-    Variable hashTerm : term -> hash.
+    Variable h : eqType.
+    Variable hashTerm : term -> h.
+
+    (* Record hinput := mkHinput { *)
+    (*                     A : Type; *)
+    (*                     input : A ; *)
+    (*                     output : h ; *)
+    (*                     f : A -> h; *)
+    (*                     (* heqin : f input == output *) *)
+    (*                   }. *)
+
+    Record hi_term :=
+      mkHinput {
+          input : term;
+          output : h ;
+          io : hashTerm input == output 
+        }.
+
+    (* Definition hi_triple (t : triple) := *)
+    (*   {| *)
+    (*       A := triple; *)
+    (*       input := t; *)
+    (*       output := hashTriple t; *)
+    (*       f := hashTriple; *)
+    (*   |}. *)
+
     Hypothesis perfectHashingSchemeTerm : injective hashTerm.
+
+    Lemma by_perf_hash (i : term) (o : h) (eqb : hashTerm i == o) : hashTerm i = o. apply /eqP. apply eqb. Qed.
+
+    Definition hi_term_inj (hin1 hin2: hi_term):
+      output hin1 = output hin2 ->
+      hin1 = hin2.
+    Proof. case: hin1; case: hin2 => [i1 o1 io1] i2 o2 io2 /= oeq. 
+           have ieq : i1 = i2.
+           apply perfectHashingSchemeTerm; apply /eqP; by rewrite (by_perf_hash io1) (by_perf_hash io2) oeq.
+           subst. by f_equal; apply eq_irrelevance.
+    Qed.
+
+    Definition eqb_hi_term (hin1 hin2: hi_term) : bool :=
+      output hin1 == output hin2.
+
+    Lemma hi_term_eqP : Equality.axiom eqb_hi_term.
+    Proof.
+      rewrite /Equality.axiom => x y.
+      apply: (iffP idP) => //= [| ->]; rewrite /eqb_hi_term.
+      case: x; case: y => [ix ox iox] iy oy ioy /= eq. apply hi_term_inj. rewrite /=. apply /eqP. apply eq.
+      by [].
+    Qed.
+
+    Canonical hi_term_eqType := EqType hi_term (EqMixin hi_term_eqP).
+    (* Inductive hit (t : term) : h -> Type := *)
+    (* | ha : hit t (hashTerm t). *)
+
+    (* Definition hit_eq (t : term) : (hit t (hashTerm t)) := *)
+    (*   (ha t).  *)
+
+    Definition hash := option hi_term.
+
+    (* Definition eqb_hash (h1 h2: hash) := *)
+    (*   match h1, h2 with *)
+    (*   | None,None => true *)
+    (*   | Some hin1,Some hin2 => hin1 == hin2 *)
+    (*   | _,_ => false *)
+    (*   end. *)
+
+    Canonical hash_eqType := EqType hash [eqMixin of hash].
+
+
+    (* Definition initTerm (t : term) : hash := *)
+    (*   match t with *)
+    (*   | Bnode name => None *)
+    (*   | otherwise => Some (hi_term t) end. *)
+
+    Definition hashmap := seq hash.
+
+    (* Definition initHashMap (g : rdf_graph) : hashmap := map initTerm (terms g). *)
+    (* Variable doHash (g : rdf_graph) (hm : hashmap) (hm : seq hashmap) (n : nat) -> seq hashmap. *)
+
+    Variable hashNodes : (rdf_graph -> seq hashmap).
+    Variable lookup_hashmap : (hashmap -> term -> hash).
+
+    (* Let nth := nth hashmap [::]. *)
+
+    Hypothesis hash_dont_get_equal : forall (g : rdf_graph) (hms : seq hashmap)
+                                       (ghashh : hashNodes g = hms)
+                                       (i j : nat) (ileqj : i <= j) (lim : j < size hms)
+                                       (x y : term) (bnx : is_bnode x) (bny : is_bnode y)
+                                       (xing : x \in (terms g)) (ying : y \in (terms g)),
+        (lookup_hashmap (nth [::] hms i) x != lookup_hashmap (nth [::] hms i) y)
+        -> lookup_hashmap (nth [::] hms j) x != lookup_hashmap (nth [::] hms j) y. 
+
+    (* Hypothesis perfectHashingSchemeTriple : injective hashTriple. *)
+
     Variable hashBag : (seq hash -> hash).
     Hypothesis hashBag_assoc : forall (l l1 l2 l3: seq hash) (perm : l = l1 ++ l2 ++ l3),
         hashBag ([:: hashBag (l1 ++ l2)] ++ l3) = hashBag (l1 ++ [:: hashBag (l2 ++ l3)]).
     Hypothesis hashBag_comm : forall (l l1 l2: seq hash) (perm : l = l1 ++ l2),
         hashBag l = hashBag (l2 ++ l1).
+
   End IsoCanAlgorithm.
   (* Hypothesis rdf_total_order   *)
-
-
-
-
-
-
 
 End IsoCan.
